Adding lemmas for insertion

AVL.fst
@@ -8,7 +8,7 @@ type tree =
 val all_tree : f:(int-> Tot bool) -> tree -> Tot bool
 let rec all_tree f = function
     | Leaf -> true
-    | (Node k l r _) -> f k && all_tree f l && all_tree f r 
+    | (Node k l r _) -> f k && all_tree f l && all_tree f r
 
 val in_tree : x:int -> t:tree -> Tot bool
 let rec in_tree x = function
@@ -16,14 +16,14 @@ let rec in_tree x = function
   | Node y l r _ -> y = x || in_tree x l || in_tree x r
 
 val all_more_than : k:int -> t:tree -> Tot bool
-let rec all_more_than k = function 
+let rec all_more_than k = function
 | Leaf -> true
-| Node y l r _ -> y > k && all_more_than k l && all_more_than k r 
+| Node y l r _ -> y > k && all_more_than k l && all_more_than k r
 
 val all_less_than : k:int -> t:tree -> Tot (r:bool {r <==> (forall x. in_tree x t ==> x < k)})
-let rec all_less_than k = function 
+let rec all_less_than k = function
 | Leaf -> true
-| Node y l r _ -> y < k && all_less_than k l && all_less_than k r 
+| Node y l r _ -> y < k && all_less_than k l && all_less_than k r
 
 val is_bst : tree -> Tot bool
 let rec is_bst = function
@@ -37,30 +37,30 @@ val real_height : t:tree -> Tot int
 
 let rec real_height = function
   | Leaf -> 0
-  | Node _ l r _ -> 
+  | Node _ l r _ ->
     let hl = real_height l in
     let hr = real_height r in
-    1 + max hl hr 
+    1 + max hl hr
 
 val node_height : tree -> tree -> Tot int
-let node_height l r = 
+let node_height l r =
   let hl = real_height l in
   let hr = real_height r in
-  1 + max hl hr 
+  1 + max hl hr
 
 val is_real_h : int -> tree -> tree -> Tot bool
 let is_real_h v l r = v = node_height l r
 
 val has_real_heights : tree -> Tot bool
-let rec has_real_heights = function 
+let rec has_real_heights = function
   | Leaf -> true
   | Node _ l r ah -> is_real_h ah l r && has_real_heights l && has_real_heights r
 
 val get_height : t:tree {has_real_heights t} -> Tot int
 let get_height = function
     |Leaf -> 0
-    | Node _ _ _ h -> h  
-    
+    | Node _ _ _ h -> h
+
 val has_bal : int -> tree -> tree -> Tot bool
 let has_bal x l r =
   let d = real_height l - real_height r in
@@ -77,10 +77,10 @@ let is_avl t = is_bst t && has_real_heights t && is_bal t
 type avl = t:tree {is_avl t}
 
 (* trees of height N *)
-type avln (n:int) = t:avl {real_height t = n} 
+type avln (n:int) = t:avl {real_height t = n}
 (* trees of height equal to that of another T *)
 type avlt (t:tree) = t':avln (real_height t)
-type avll (k:int) = t:avl {all_less_than k t} 
+type avll (k:int) = t:avl {all_less_than k t}
 (* trees of height equal to that of another T *)
 type avlr (k:int) = t:avl {all_more_than k t}
 
@@ -91,11 +91,11 @@ val singleton : int -> avln 1
 let singleton x =  Node x empty empty 1
 
 val mk_node : v:int -> l:(avll v) -> r:avlr v {has_bal 1 l r} -> Tot (avln (node_height l r ))
-let mk_node v l r = 
+let mk_node v l r =
  let hl = get_height l in
  let hr = get_height r in
  let h = 1 + max hl hr in
-   Node v l r h 
+   Node v l r h
 
 val is_empty : t:tree -> Tot bool
 let is_empty = function
@@ -109,7 +109,7 @@ val head: t:tree {not_empty t} -> Tot int
 let head (Node x _ _ _) = x
 
 val left: t:tree {not_empty t} -> Tot tree
-let left (Node _ l _ _) = l 
+let left (Node _ l _ _) = l
 
 val right: t:tree {not_empty t} -> Tot tree
 let right (Node _ _ r _) = r
@@ -121,20 +121,20 @@ let left_of_avl_is_avll t y = ()
 val insert : x:int -> t:avl -> Tot avl
 let rec insert x = function
   | Leaf -> singleton x
-  | Node y l r h -> 
-    if x < y 
+  | Node y l r h ->
+    if x < y
     then begin
       left_of_avl_is_avll (Node y l r h) y;
       mk_node y (insert x l) r
-    end 
+    end
     else mk_node y l (insert x r)
 *)
 
-val diff : s:tree {has_real_heights s} -> t:tree {has_real_heights t} -> Tot int 
+val diff : s:tree {has_real_heights s} -> t:tree {has_real_heights t} -> Tot (r:int {get_height s <= get_height t + r } )
 let diff s t = get_height s - get_height t
 
 val get_balfac : t:tree {has_real_heights t} -> Tot int
-let get_balfac = function 
+let get_balfac = function
   | Leaf -> 0
   | Node _ l r _ -> diff l r
 
@@ -147,7 +147,7 @@ let is_right_heavy t = get_balfac t < 0
 val is_not_heavy : t:tree {has_real_heights t} -> Tot bool
 let is_not_heavy t = get_balfac t = 0
 
-val is_left_big: l:tree{has_real_heights l} -> r:tree{has_real_heights r} -> Tot bool 
+val is_left_big: l:tree{has_real_heights l} -> r:tree{has_real_heights r} -> Tot bool
 let is_left_big l r = diff l r = 2
 
 val is_right_big : l:tree{has_real_heights l} -> r:tree{has_real_heights r} -> Tot bool
@@ -166,8 +166,8 @@ val all_less_intro: v:int -> x:int {x < v} -> l:avll x {all_less_than v l} -> r:
 let all_less_intro v x l r  = ()
 
 val balL0 : x:int -> l:avll x {is_not_heavy l} -> r:avlr x {is_left_big l r} -> avln (real_height l + 1)
-let balL0 x l r = match l with 
-  | (Node lv ll lr _) -> 
+let balL0 x l r = match l with
+  | (Node lv ll lr _) ->
     let y = mk_node x lr r in
     all_more_transitive lv x r;
     mk_node lv ll y
@@ -178,67 +178,67 @@ let balLL v (Node lv ll lr _) r =
   all_more_transitive lv v r;
   mk_node lv ll (mk_node v lr r)
 
-val eq_or_up : s:tree{has_real_heights s} -> t:tree{has_real_heights t} -> Tot bool
-let eq_or_up s t = 
+val eq_or_up : s:tree{has_real_heights s} -> t:tree{has_real_heights t} -> Tot (r:bool {r <==> diff t s = 0 \/ diff t s = 1})
+let eq_or_up s t =
   let d = diff t s in
   d = 0 || d = 1
 
 val bal_ht : l:tree -> r:tree -> t:tree -> Tot bool
 let bal_ht l r t = not (has_bal 1 l r) || is_real_h (real_height t) l r
 
-val big_ht : l:tree{has_real_heights l} -> r:tree{has_real_heights r} -> t:tree{has_real_heights t} -> Tot bool 
-let big_ht l r t = 
+val big_ht : l:tree{has_real_heights l} -> r:tree{has_real_heights r} -> t:tree{has_real_heights t} -> Tot bool
+let big_ht l r t =
   let hl = real_height l in
   let hr = real_height r in
   let l_big    = not (hl >= hr) || (eq_or_up l t) in
   let r_big    = (hl >= hr)     || (eq_or_up r t) in
   l_big && r_big
 
-val re_bal : l:tree {has_real_heights l} -> r:tree {has_real_heights r} -> t:tree{has_real_heights t} -> Tot bool  
+val re_bal : l:tree {has_real_heights l} -> r:tree {has_real_heights r} -> t:tree{has_real_heights t} -> Tot bool
 let re_bal l r t = big_ht l r t && bal_ht l r t
 
 val balLR :x:int  -> l:avll x {is_right_heavy l} -> r:avlr x {is_left_big l r} -> Tot (avlt l)
 let balLR v l r = match l with
-  | (Node lv ll (Node lrv lrl lrr lrh) lh) -> 
+  | (Node lv ll (Node lrv lrl lrr lrh) lh) ->
     let y = mk_node v lrr r in
-       
+
     all_more_transitive lrv v r;
-    all_less_transitive lrv lv ll; 
+    all_less_transitive lrv lv ll;
 
     mk_node lrv (mk_node lv ll lrl) (y)
-  | _ -> 
+  | _ ->
     (* should be impossible *)
     admit()
 
 
 val balR0 : x:int  -> r:avlr x {is_not_heavy r} -> l:avll x {is_right_big l r} -> Tot (avln (real_height r + 1))
-let balR0 x r l = match r with 
+let balR0 x r l = match r with
   | (Node rv rl rr _) ->
     all_less_transitive rv x l;
     mk_node rv (mk_node x l rl) rr
-  | _ -> 
+  | _ ->
    (* should be impossible *)
     admit ()
 
 
 val balRR : x:int -> l:avll x -> r:avlr x {is_right_big l r && is_right_heavy r} -> Tot (avlt r)
-let balRR x l (Node rv rl rr _) = 
+let balRR x l (Node rv rl rr _) =
   all_less_transitive rv x l;
-  mk_node rv (mk_node x l rl) rr 
+  mk_node rv (mk_node x l rl) rr
 
 val balRL : x:int -> l: avll x -> r:avlr x {is_right_big l r && is_left_heavy r} -> Tot (avlt r)
 let balRL x l = function
-  | (Node rv (Node rlv rll rlr _) rr _) -> 
+  | (Node rv (Node rlv rll rlr _) rr _) ->
     all_less_transitive rlv x l;
     all_more_transitive rlv rv rr;
     mk_node rlv (mk_node x l rll ) (mk_node rv rlr rr)
-  | _ -> 
+  | _ ->
     (* should be impossible *)
     admit ()
 
 
-val bal : x:int -> l:avll x -> r:avlr x {has_bal 2 l r} -> t:avl {re_bal l r t}
-let bal v l r  = 
+val bal : x:int -> l:avll x -> r:avlr x {has_bal 2 l r} -> t:avl {re_bal l r t /\ (forall y. in_tree y t <==> in_tree y l \/ in_tree y r \/ x = y)}
+let bal v l r  =
   admit ();
   let ilb = is_left_big l r in
   let irb = is_right_big l r in
@@ -251,14 +251,14 @@ let bal v l r  =
   else mk_node v l r
 
 val minimum : t:tree {not_empty t} -> Tot int
-let rec minimum (Node x l r _) = 
+let rec minimum (Node x l r _) =
   let lv = if not_empty l then minimum l else x in
   let lr = if not_empty r then minimum r else x in
   min( min x lv) lr
 
 
 val maximum : t:tree {not_empty t} -> Tot int
-let rec maximum (Node x l r _) = 
+let rec maximum (Node x l r _) =
   let lv = if not_empty l then maximum l else x in
   let lr = if not_empty r then maximum r else x in
   max ( max x lv) lr
@@ -317,17 +317,36 @@ let rec insert_bst x t =
                       Node n t1 (insert_bst x t2) (node_height t1 (insert_bst x t2))
                     end
 
+val bal_not_empty : x:int -> l:avll x -> r:avlr x {has_bal 2 l r} -> Lemma (not_empty (bal x l r))
+let bal_not_empty x l r = ()
 
-val insert: x:int -> s:avl -> Tot (t:avl {not_empty t /\ eq_or_up s t /\ (forall y. in_tree y t <==> (in_tree y s \/ x = y))})
+val bal_height : x:int -> l:avll x -> r:avlr x {has_bal 2 l r} -> Lemma (real_height (bal x l r) = node_height l r \/ real_height (bal x l r) = node_height l r - 1)
+let bal_height x l r = ()
+
+val bal_in_tree : x:int -> l:avll x -> r:avlr x {has_bal 2 l r} -> Lemma (forall y. in_tree y (bal x l r) <==> in_tree y l \/ in_tree y r \/ x = y)
+let bal_in_tree x l r = ()
+
+
+val insert: x:int -> s:avl -> Tot (t:avl {not_empty t /\ eq_or_up s t /\ (forall y. (in_tree y t) <==> (in_tree y s \/ x = y))})
 let rec insert x s = match s with
   | Leaf -> singleton x
-  | Node v l r _ -> 
+  | Node v l r _ ->
     if x < v then begin
       let insl = insert x l in
       less_than_in_tree_lemma v l;
       in_tree_less_than_lemma v insl;
-       
-      bal v insl r
+      bal_not_empty v insl r;
+      bal_height v insl r;
+      bal_in_tree v insl r;
+      assert (is_avl (bal v insl r));
+      assert (eq_or_up l insl);
+      assert (real_height s <= real_height (bal v insl r));
+      assert (real_height (bal v insl r) <= real_height s + 1);
+      assert (real_height (bal v insl r) - real_height s <= 1);
+      assert (diff (bal v insl r) s = 0 \/ diff (bal v insl r) s = 1);
+      assert (eq_or_up s (bal v insl r));
+      assert ( (forall y. (in_tree y insl) <==> (in_tree y l \/ x = y)));
+      admit ()
     end else if x > v then begin
       admit ()
     end else s
